Clean

NuSys.thy
@@ -300,7 +300,7 @@ datatype uniq_id = UNIQ_ID
   \<comment> \<open>A technical tag that is during the exporting translated to a unique ID.
     It is useful to generate unique name of anonymous functions.\<close>
 
-subsubsection \<open>Different tag\<close>
+subsubsection \<open>The Different Tag\<close>
 
 definition Different :: " 'a \<Rightarrow> 'b \<Rightarrow> bool " where "Different A B = True"
   \<comment> \<open>A premise that solved by automatic reasoning only if the term expressions of A and B
@@ -504,54 +504,17 @@ subsection \<open>Miscellaneous\<close>
 
 subsubsection \<open>Finalization Rewrites\<close>
 
-named_theorems final_proc_rewrite \<open>rewrite the generated procedure theorem in the final stage\<close>
+named_theorems final_proc_rewrite
+  \<open>Rewrite the specification theorem in the end of the construction.
+    Theorems should be a meta equition \<^term>\<open>\<equiv>\<close>.\<close>
 
 lemma [final_proc_rewrite]: "f \<then> nop \<equiv> f" and [final_proc_rewrite]: "nop \<then> f \<equiv> f"
   unfolding instr_comp_def nop_def bind_def atomize_eq by auto
 
-(* lemmas [final_proc_rewrite] = WorkingProtector_def *)
 
 section \<open>Syntax\<close>
 
-subsection \<open>Syntax Helper\<close>
-
-ML \<open>
-fun parse_typing_ty (Type (\<^type_name>\<open>typing\<close>, [a,b])) = (b, a --> b --> \<^typ>\<open>bool\<close>)
-  | parse_typing_ty dummyT = (dummyT, dummyT)
-  | parse_typing_ty ty = raise TYPE ("should be a typing type", [ty], [])
-
-fun parse_typing (Free (name, ty)) =
-    Const (\<^const_syntax>\<open>typing\<close>, ty) $ Free (name^"\<^sub>x", fst (parse_typing_ty ty))
-        $ Free (name^"\<^sub>t\<^sub>y", snd (parse_typing_ty ty))
-  | parse_typing (Var ((name,ind), ty)) =
-    Const (\<^const_syntax>\<open>typing\<close>, ty) $ Var ((name^"\<^sub>x",ind), fst (parse_typing_ty ty))
-        $ Var ((name^"\<^sub>t\<^sub>y", ind), snd (parse_typing_ty ty))
-  | parse_typing (Const (\<^syntax_const>\<open>_constrain\<close>, ty) $ tm $ (Const (\<^type_syntax>\<open>typing\<close>, _) $ tya $ tyb)) =
-      let val (const $ tmx $ tmty) = parse_typing tm
-      in const $ (Const (\<^syntax_const>\<open>_constrain\<close>, ty) $ tmx $ tyb)
-        $ (Const (\<^syntax_const>\<open>_constrain\<close>, ty) $ tmty $ (Const (\<^type_syntax>\<open>\<nu>\<close>, dummyT) $ tya $ tyb)) end
-  | parse_typing (Const (\<^syntax_const>\<open>_constrain\<close>, ty) $ tm $ markup) =
-      let val (const $ tmx $ tmty) = parse_typing tm
-      in const $ (Const (\<^syntax_const>\<open>_constrain\<close>, ty) $ tmx $ markup)
-        $ (Const (\<^syntax_const>\<open>_constrain\<close>, ty) $ tmty $ markup) end
-  | parse_typing (tm as Const (\<^const_syntax>\<open>typing\<close>, _) $ _ $ _) = tm
-  | parse_typing tm = raise TERM ("should be a NuPrime.typing term", [tm])
-
-fun parse_typing_x tm = (case parse_typing tm of _ $ x $ _ => x)
-fun parse_typing_ty tm = (case parse_typing tm of _ $ _ $ ty => ty)
-\<close>
-
-syntax "_\<nu>typing" :: " logic \<Rightarrow> logic "
-  "_\<nu>typing_x" :: " logic \<Rightarrow> logic "
-  "_\<nu>typing_ty" :: " logic \<Rightarrow> logic "
-parse_translation \<open>[
-  (\<^syntax_const>\<open>_\<nu>typing\<close>, (fn _ => fn [tm] => parse_typing tm)),
-  (\<^syntax_const>\<open>_\<nu>typing_x\<close>, (fn _ => fn [tm] => parse_typing_x tm)),
-  (\<^syntax_const>\<open>_\<nu>typing_ty\<close>, (fn _ => fn [tm] => parse_typing_ty tm))
-]\<close>
-
-
-subsection \<open>Logical image models\<close>
+subsection \<open>Logical Image Models\<close>
 
 text \<open>A set of models having common meanings, useful for representing logical images\<close>
 
@@ -631,7 +594,6 @@ lemma [nu_exps]: "h \<nuLinkL> A \<^emph> B \<nuLinkR> (a,b) \<longleftrightarro
   (\<exists>h2 h1. h = h2 ++ h1 \<and> dom h2 \<perpendicular> dom h1 \<and> (h1 \<nuLinkL> A \<nuLinkR> a) \<and> (h2 \<nuLinkL> B \<nuLinkR> b))"
   unfolding HeapSeparation_def Refining_def by simp
 
-
 lemma SepNu_to_SepSet: "(OBJ (a,b) \<tycolon> A \<^emph> B) = (a \<tycolon> A \<heavy_asterisk> b \<tycolon> B)"
   by (simp add: nu_exps set_eq_iff) blast
 
@@ -645,9 +607,8 @@ lemma heap_split_by_addr_set: "P (h |` (MemAddress ` S)) (h |` (- (MemAddress ` 
   using heap_split_by_set .
 
 
-subsection \<open>Fusion and its derivatives\<close>
+subsection \<open>Fusion\<close>
 
-subsubsection \<open>Fusion\<close>
 
 definition Fusion :: "('a1,'b1) \<nu> \<Rightarrow> ('a2,'b2) \<nu> \<Rightarrow> ('a1 \<times> 'a2, 'b1 \<times> 'b2) \<nu>" (infixr "\<cross_product>" 70) 
   where "Fusion N M x = {(p1,p2). case x of (x1,x2) \<Rightarrow> (p1 \<nuLinkL> N \<nuLinkR> x1) \<and> (p2 \<nuLinkL> M \<nuLinkR> x2)}"
@@ -706,6 +667,26 @@ translations "\<exists>* idts. x \<tycolon> T" \<rightleftharpoons> "\<exists>* 
 
 lemma [nu_exps]: "p \<in> ExSet S \<longleftrightarrow> (\<exists>c. p \<in> S c)" unfolding ExSet_def by simp
 
+syntax
+  "_SetcomprNu" :: "'a \<Rightarrow> idts \<Rightarrow> bool \<Rightarrow> 'a set"  ("_ \<^bold>s\<^bold>u\<^bold>b\<^bold>j/ _./ _ " [2,0,2] 2)
+
+translations
+  " X \<^bold>s\<^bold>u\<^bold>b\<^bold>j idts. P " \<rightleftharpoons> "\<exists>* idts. X \<^bold>s\<^bold>u\<^bold>b\<^bold>j P"
+  " X \<^bold>s\<^bold>u\<^bold>b\<^bold>j idts. P " <= " \<tort_lbrace> X \<tort_rbrace> \<^bold>s\<^bold>u\<^bold>b\<^bold>j idts. P "
+  " X \<^bold>s\<^bold>u\<^bold>b\<^bold>j idts. CONST True " \<rightleftharpoons> "\<exists>* idts. X"
+
+translations
+  "\<^bold>p\<^bold>r\<^bold>o\<^bold>c f \<blangle> a \<tycolon> A \<^bold>s\<^bold>u\<^bold>b\<^bold>j idts. P \<longmapsto> B \<brangle>" \<rightleftharpoons> "\<^bold>p\<^bold>r\<^bold>o\<^bold>c f \<blangle> CONST Ele \<tort_lbrace> a \<tycolon> A \<tort_rbrace> \<^bold>s\<^bold>u\<^bold>b\<^bold>j idts. P \<longmapsto> B \<brangle>"
+  "\<^bold>p\<^bold>r\<^bold>o\<^bold>c f \<blangle> A \<longmapsto> b \<tycolon> B \<^bold>s\<^bold>u\<^bold>b\<^bold>j idts. Q \<brangle>" \<rightleftharpoons> "\<^bold>p\<^bold>r\<^bold>o\<^bold>c f \<blangle> A \<longmapsto> CONST Ele \<tort_lbrace> b \<tycolon> B \<tort_rbrace> \<^bold>s\<^bold>u\<^bold>b\<^bold>j idts. Q \<brangle>"
+
+text \<open>The set of \<nu>-type in an assertion like \<^term>\<open>\<^bold>p\<^bold>r\<^bold>o\<^bold>c f \<blangle> S x \<^bold>s\<^bold>u\<^bold>b\<^bold>j x. P x \<longmapsto> T x \<^bold>s\<^bold>u\<^bold>b\<^bold>j x. Q x \<brangle>\<close> is represented
+  by \<^const>\<open>ExSet\<close> and we show a \<nu>-type \<^term>\<open>S x \<^bold>s\<^bold>u\<^bold>b\<^bold>j x. P x\<close> represents actually all concrete values that
+  belongs to \<^term>\<open>S\<close> a set of \<nu>-types (i.e. the union of \<^term>\<open>S\<close>) by following lemma\<close>
+
+lemma " Union { S x |x. P x } = (S x \<^bold>s\<^bold>u\<^bold>b\<^bold>j x. P x) "
+  by (simp add: set_eq_iff nu_exps) blast
+
+
 lemma ExSet_pair: "ExSet T = (\<exists>*c1 c2. T (c1,c2) )" by (auto simp add: nu_exps)
 lemma named_ExSet: "(ExSet T) = (\<exists>*c. T (tag c) )" by (auto simp add: named_exists nu_exps)
 
@@ -730,37 +711,20 @@ lemma generalize_\<nu>app:
     \<Longrightarrow> lambda_abstraction c (T' \<^bold>s\<^bold>u\<^bold>b\<^bold>j P c) name T \<Longrightarrow> \<^bold>c\<^bold>a\<^bold>s\<^bold>t T' \<longmapsto> \<^bold>( ExSet T \<^bold>) "
   unfolding Cast_def Implicit_Protector_def lambda_abstraction_def by (auto simp add: nu_exps)
 
-syntax
-  "_SetcomprNu" :: "'a \<Rightarrow> idts \<Rightarrow> bool \<Rightarrow> 'a set"  ("_ \<^bold>s\<^bold>u\<^bold>b\<^bold>j/ _./ _ " [2,0,2] 2)
-
-translations
-  " X \<^bold>s\<^bold>u\<^bold>b\<^bold>j idts. P " \<rightleftharpoons> "\<exists>* idts. X \<^bold>s\<^bold>u\<^bold>b\<^bold>j P"
-  " X \<^bold>s\<^bold>u\<^bold>b\<^bold>j idts. P " <= " \<tort_lbrace> X \<tort_rbrace> \<^bold>s\<^bold>u\<^bold>b\<^bold>j idts. P "
-  " X \<^bold>s\<^bold>u\<^bold>b\<^bold>j idts. CONST True " \<rightleftharpoons> "\<exists>* idts. X"
-
-translations
-  "\<^bold>p\<^bold>r\<^bold>o\<^bold>c f \<blangle> a \<tycolon> A \<^bold>s\<^bold>u\<^bold>b\<^bold>j idts. P \<longmapsto> B \<brangle>" \<rightleftharpoons> "\<^bold>p\<^bold>r\<^bold>o\<^bold>c f \<blangle> CONST Ele \<tort_lbrace> a \<tycolon> A \<tort_rbrace> \<^bold>s\<^bold>u\<^bold>b\<^bold>j idts. P \<longmapsto> B \<brangle>"
-  "\<^bold>p\<^bold>r\<^bold>o\<^bold>c f \<blangle> A \<longmapsto> b \<tycolon> B \<^bold>s\<^bold>u\<^bold>b\<^bold>j idts. Q \<brangle>" \<rightleftharpoons> "\<^bold>p\<^bold>r\<^bold>o\<^bold>c f \<blangle> A \<longmapsto> CONST Ele \<tort_lbrace> b \<tycolon> B \<tort_rbrace> \<^bold>s\<^bold>u\<^bold>b\<^bold>j idts. Q \<brangle>"
-
-
-lemma " Union { S x |x. P x } = (S x \<^bold>s\<^bold>u\<^bold>b\<^bold>j x. P x) "
-  by (simp add: set_eq_iff nu_exps) blast
-
 
 subsection \<open>Identity\<close>
 
 definition Identity :: " ('a::lrep, 'a) \<nu> " where "Identity x = {x}"
 lemma [simp]: "p \<nuLinkL> Identity \<nuLinkR> x \<longleftrightarrow> p = x" unfolding Refining_def Identity_def by auto
 
+
 subsection \<open>Refinement\<close>
 
-definition NuRefine :: " ('a, 'b) \<nu> \<Rightarrow> 'b set \<Rightarrow> ('a, 'b) \<nu> " (infixl "\<nuRefine>" 80)
-  where "(N \<nuRefine> T) x = {p. (x \<in> T \<and>(p \<nuLinkL> N \<nuLinkR> x))}"
+definition NuRefine :: " ('a, 'b) \<nu> \<Rightarrow> 'b set \<Rightarrow> ('a, 'b) \<nu> " (infixl "<where>" 80)
+  where "(N <where> T) x = {p. (x \<in> T \<and>(p \<nuLinkL> N \<nuLinkR> x))}"
 
-notation NuRefine (infixl "<where>" 80)
-
-lemma [simp]: " p \<nuLinkL> N \<nuRefine> P \<nuLinkR> x \<longleftrightarrow> x \<in> P \<and> ( p \<nuLinkL> N \<nuLinkR> x)" unfolding NuRefine_def Refining_def by simp
-lemma [elim,\<nu>elim]: " x \<ratio> N \<nuRefine> P \<Longrightarrow> (x \<in> P \<Longrightarrow> x \<ratio> N \<Longrightarrow> C) \<Longrightarrow> C" unfolding Inhabited_def by (simp add: nu_exps)
+lemma [simp]: " p \<nuLinkL> N <where> P \<nuLinkR> x \<longleftrightarrow> x \<in> P \<and> ( p \<nuLinkL> N \<nuLinkR> x)" unfolding NuRefine_def Refining_def by simp
+lemma [elim,\<nu>elim]: " x \<ratio> N <where> P \<Longrightarrow> (x \<in> P \<Longrightarrow> x \<ratio> N \<Longrightarrow> C) \<Longrightarrow> C" unfolding Inhabited_def by (simp add: nu_exps)
 
 lemma [\<nu>reason]: "\<^bold>c\<^bold>a\<^bold>s\<^bold>t x \<tycolon> M \<longmapsto> x' \<tycolon> M' \<^bold>w\<^bold>i\<^bold>t\<^bold>h P \<Longrightarrow> \<^bold>p\<^bold>r\<^bold>e\<^bold>m\<^bold>i\<^bold>s\<^bold>e x' \<in> S \<Longrightarrow> \<^bold>c\<^bold>a\<^bold>s\<^bold>t x \<tycolon> M \<longmapsto> x' \<tycolon> M' <where> S \<^bold>w\<^bold>i\<^bold>t\<^bold>h P"
   unfolding Cast_def by (simp add: nu_exps) blast
@@ -772,24 +736,6 @@ lemma [\<nu>reason 30 on \<open>\<^bold>c\<^bold>a\<^bold>s\<^bold>t ?x \<tycolo
 
 lemma refine_\<nu>app: "\<^bold>p\<^bold>a\<^bold>r\<^bold>a\<^bold>m P \<Longrightarrow> \<^bold>p\<^bold>r\<^bold>e\<^bold>m\<^bold>i\<^bold>s\<^bold>e x \<in> P \<Longrightarrow> \<^bold>c\<^bold>a\<^bold>s\<^bold>t x \<tycolon> N \<longmapsto> x \<tycolon> (N <where> P)"
   unfolding Cast_def by (simp add: nu_exps) blast
-
-(* TODO: TO BE REMOVED *)
-abbreviation AutoRefine (infixl "<auto-where>" 80)
-  where "AutoRefine N P \<equiv> Auto (NuRefine N P)"
-
-lemma [simp]:"\<tort_lbrace>x \<tycolon> T <auto-where> P \<tort_rbrace> = ((x \<tycolon> T) \<^bold>s\<^bold>u\<^bold>b\<^bold>j (\<^bold>p\<^bold>r\<^bold>e\<^bold>m\<^bold>i\<^bold>s\<^bold>e x \<in> P))"
-  unfolding Auto_def Premise_def by (auto simp add: nu_exps)
-
-lemma NuRefine_to_auto:"\<tort_lbrace>x \<tycolon> T <where> P \<tort_rbrace> = \<tort_lbrace>x \<tycolon> T <auto-where> P \<tort_rbrace>" unfolding Auto_def ..
-
-(* lemma [\<nu>intro]: "(x \<in> P \<Longrightarrow> \<^bold>c\<^bold>a\<^bold>s\<^bold>t x \<tycolon> N \<longmapsto> Y \<^bold>w\<^bold>i\<^bold>t\<^bold>h Q) \<Longrightarrow> \<^bold>c\<^bold>a\<^bold>s\<^bold>t x \<tycolon> N \<nuRefine> P \<longmapsto> Y \<^bold>w\<^bold>i\<^bold>t\<^bold>h Q \<and>x \<in> P" unfolding Cast_def by auto
-lemma [\<nu>intro]: " \<^bold>c\<^bold>a\<^bold>s\<^bold>t x \<tycolon> N \<longmapsto> y \<tycolon> M \<^bold>w\<^bold>i\<^bold>t\<^bold>h Q \<Longrightarrow> \<^bold>p\<^bold>r\<^bold>e\<^bold>m\<^bold>i\<^bold>s\<^bold>e y \<in> P \<Longrightarrow> \<^bold>c\<^bold>a\<^bold>s\<^bold>t x \<tycolon> N \<longmapsto> y \<tycolon> M <where> P \<^bold>w\<^bold>i\<^bold>t\<^bold>h Q" unfolding Cast_def by auto
-(* lemma [\<nu>cast_overload E]: " \<^bold>c\<^bold>a\<^bold>s\<^bold>t x \<tycolon> (N \<^bold>w\<^bold>h\<^bold>e\<^bold>r\<^bold>e P) \<longmapsto> x \<tycolon> N \<^bold>w\<^bold>i\<^bold>t\<^bold>h x \<in> P" unfolding Cast_def by auto *)
-*)
-lemma [\<nu>reason]: "\<^bold>p\<^bold>r\<^bold>e\<^bold>m\<^bold>i\<^bold>s\<^bold>e z \<in> S \<Longrightarrow> \<nu>Zero N z \<Longrightarrow> \<nu>Zero (N <where> S) z"
-  unfolding \<nu>Zero_def Premise_def by (simp add: nu_exps)
-lemma "\<nu>Equal (N <where> P) can_eq eq \<longleftrightarrow> \<nu>Equal N (\<lambda>x y. x \<in> P \<and> y \<in> P \<and> can_eq x y) eq"
-  unfolding \<nu>Equal_def by (simp add: nu_exps) blast
 
 
 subsection \<open>Down Lifting\<close>
