NuHelpMath.thy
@@ -11,4 +11,5 @@ lemma pair_forall: "All P \<longleftrightarrow> (\<forall>a b. P (a,b))" using s
 lemmas pair_All = split_paired_all
 
 lemma conj_imp: "(P \<and> Q \<Longrightarrow> PROP R) \<equiv> (P \<Longrightarrow> Q \<Longrightarrow> PROP R)" by rule simp+
+
 end
